Improving state monad to be COOL

theories/StateMonad.v
@@ -2,32 +2,22 @@ From Stdlib Require Import List.
 From RocqCandy Require Import Tactics ResultMonad.
 
 (* State Monad definition *)
-Inductive State (St A E : Type) : Type :=
-| state : (St -> (Result A E * St)) -> State St A E.
-Arguments state {St A E} _.
+Definition State (St A E : Type) : Type := (St -> (Result A E * St))%type.
 
 (* Monadic bind for State *)
 Definition state_bind {St A B E} (m : State St A E) (f : A -> State St B E) : State St B E :=
-  state (fun s =>
-    let '(a, s') := match m with state run => run s end in
+  fun s =>
+    let '(a, s') := m s in
     match a with
-    | res a => match f a with state run' => run' s' end
+    | res a => f a s'
     | err e => (err e, s')
-    end).
-
-(* Run a stateful computation *)
-Definition run_state {St A E} (m : State St A E) (init : St) : (Result A E * St) :=
-  match m with state run => run init end.
+    end.
 
 (* Get and put operations *)
-Definition get {St E} : State St St E := 
-  state (fun s => (res s, s)).
-Definition put {St E} (s : St) : State St unit E := 
-  state (fun _ => (res tt, s)).
-Definition ret {St A E} (a : A) : State St A E := 
-  state (fun s => (res a, s)).
-Definition fail {St A E} (e : E) : State St A E := 
-  state (fun s => (err e, s)).
+Definition get {St E} : State St St E := fun s => (res s, s).
+Definition put {St E} (s : St) : State St unit E := fun _ => (res tt, s).
+Definition ret {St A E} (a : A) : State St A E := fun s => (res a, s).
+Definition fail {St A E} (e : E) : State St A E := fun s => (err e, s).
 
 (* Notation scope for State Monad *)
 Module Export StateNotation.
@@ -38,7 +28,6 @@ Module Export StateNotation.
     (at level 61, pat pattern, m at next level, right associativity).
   Notation "e1 ;;; e2" := (_ <~ e1 ;;; e2) (at level 61, right associativity).
   Global Hint Unfold state_bind : core.
-  Global Hint Unfold run_state : core.
   Global Hint Unfold get put ret fail : core.
 End StateNotation.
 Export StateNotation.
@@ -46,17 +35,17 @@ Export StateNotation.
 (* Map over a list in the State monad *)
 Fixpoint state_map {St A B E} (f : A -> State St B E) (l : list A) : State St (list B) E :=
   match l with
-  | nil => state (fun s => (res nil, s))
+  | nil => fun s => (res nil, s)
   | cons h t =>
     v <~ f h ;;;
     vs <~ state_map f t ;;;
-    state (fun s => (res (v :: vs), s))
+    ret (v :: vs)
   end.
 
 (* Fold over a list in the State monad *)
 Fixpoint state_fold {St A B E} (f : A -> B -> State St B E) (acc : B) (l : list A) : State St B E :=
   match l with
-  | nil => state (fun s => (res acc, s))
+  | nil => fun s => (res acc, s)
   | cons h t =>
     acc' <~ f h acc ;;;
     state_fold f acc' t
@@ -64,19 +53,19 @@ Fixpoint state_fold {St A B E} (f : A -> B -> State St B E) (acc : B) (l : list 
 
 (* Theorems about State Monad *)
 Lemma state_bind_left_id : forall St A B E (a : A) (f : A -> State St B E) init,
-  run_state (state_bind (state (fun s => (res a, s))) f) init = run_state (f a) init.
+  state_bind (ret a) f init = (f a) init.
 Proof.
   ff.
 Qed.
 
 Lemma state_bind_right_id : forall St A E (m : State St A E) init,
-  run_state (state_bind m (fun a => state (fun s => (res a, s)))) init = run_state m init.
+  (state_bind m (fun a => (fun s => (res a, s)))) init = m init.
 Proof.
-  ff.
+  ff u.
 Qed.
 
 Lemma state_bind_assoc : forall St A B C E (m : State St A E) (f : A -> State St B E) (g : B -> State St C E) init,
-  run_state (state_bind (state_bind m f) g) init = run_state (state_bind m (fun x => state_bind (f x) g)) init.
+  state_bind (state_bind m f) g init = state_bind m (fun x => state_bind (f x) g) init.
 Proof.
-  ff.
+  ff u.
 Qed.
